resolving some pull request comments + a few smts removed

BoogieLang/Ast.thy
@@ -84,9 +84,9 @@ fun is_final :: "'a ast_config \<Rightarrow> bool"
 
 text\<open>function defining the semantics of bigblocks; small-step semantics 
       Note: arrow symbols in the 'syntactic sugar' clash if the exact same syntax is used as in red_cmd\<close>
-inductive red_bigblock :: "'a absval_ty_fun \<Rightarrow> ast proc_context \<Rightarrow> var_context \<Rightarrow> 'a fun_interp \<Rightarrow> rtype_env  \<Rightarrow> ast \<Rightarrow> 'a ast_config \<Rightarrow> 'a ast_config \<Rightarrow> bool" 
+inductive red_bigblock :: "'a absval_ty_fun \<Rightarrow> 'm proc_context \<Rightarrow> var_context \<Rightarrow> 'a fun_interp \<Rightarrow> rtype_env  \<Rightarrow> ast \<Rightarrow> 'a ast_config \<Rightarrow> 'a ast_config \<Rightarrow> bool" 
   ("_,_,_,_,_,_ \<turnstile> (\<langle>_\<rangle> \<longrightarrow>/ _)" [51,0,0,0] 81)
-  for A :: "'a absval_ty_fun" and M :: "ast proc_context" and \<Lambda> :: var_context and \<Gamma> :: "'a fun_interp" and \<Omega> :: rtype_env and T :: ast
+  for A :: "'a absval_ty_fun" and M :: "'m proc_context" and \<Lambda> :: var_context and \<Gamma> :: "'a fun_interp" and \<Omega> :: rtype_env and T :: ast
   where
     RedSimpleCmds: 
     "\<lbrakk>(A,M,\<Lambda>,\<Gamma>,\<Omega> \<turnstile> \<langle>cs, (Normal n_s)\<rangle> [\<rightarrow>] s1) \<and> (cs \<noteq> Nil) \<rbrakk> 
@@ -188,7 +188,7 @@ inductive red_bigblock :: "'a absval_ty_fun \<Rightarrow> ast proc_context \<Rig
         \<Longrightarrow> A,M,\<Lambda>,\<Gamma>,\<Omega>,T \<turnstile> \<langle>((BigBlock bb_name [] None (Some (Goto label))), cont0, Normal n_s)\<rangle> \<longrightarrow> 
                             (found_bigblock, found_cont, (Normal n_s))"
 
-abbreviation red_bigblock_k_step :: "'a absval_ty_fun \<Rightarrow> ast proc_context \<Rightarrow> var_context \<Rightarrow> 'a fun_interp \<Rightarrow> rtype_env \<Rightarrow> ast \<Rightarrow> 'a ast_config \<Rightarrow> nat \<Rightarrow> 'a ast_config \<Rightarrow> bool"
+abbreviation red_bigblock_k_step :: "'a absval_ty_fun \<Rightarrow> 'm proc_context \<Rightarrow> var_context \<Rightarrow> 'a fun_interp \<Rightarrow> rtype_env \<Rightarrow> ast \<Rightarrow> 'a ast_config \<Rightarrow> nat \<Rightarrow> 'a ast_config \<Rightarrow> bool"
   ("_,_,_,_,_,_ \<turnstile>_ -n\<longrightarrow>^_/ _" [51,0,0,0,0] 81)
 where "red_bigblock_k_step A M \<Lambda> \<Gamma> \<Omega> T c1 n c2 \<equiv> ((red_bigblock A M \<Lambda> \<Gamma> \<Omega> T)^^n) c1 c2"
 
@@ -203,10 +203,10 @@ fun init_ast :: "ast \<Rightarrow> 'a nstate \<Rightarrow> 'a ast_config"
 
 definition valid_configuration 
   where "valid_configuration A \<Lambda> \<Gamma> \<Omega> posts bb cont state \<equiv> 
-         (get_state (bb, cont, state)) \<noteq> Failure \<and> 
-         (is_final (bb, cont, state) \<longrightarrow> (\<forall>ns'. (get_state (bb, cont, state)) = Normal ns' \<longrightarrow> expr_all_sat A \<Lambda> \<Gamma> \<Omega> ns' posts))"
+         state \<noteq> Failure \<and> 
+         (is_final (bb, cont, state) \<longrightarrow> (\<forall>ns'. state = Normal ns' \<longrightarrow> expr_all_sat A \<Lambda> \<Gamma> \<Omega> ns' posts))"
 
-definition proc_body_satisfies_spec :: "'a absval_ty_fun \<Rightarrow> ast proc_context \<Rightarrow> var_context \<Rightarrow> 'a fun_interp \<Rightarrow> rtype_env \<Rightarrow> expr list \<Rightarrow> expr list \<Rightarrow> ast \<Rightarrow> 'a nstate \<Rightarrow> bool"
+definition proc_body_satisfies_spec :: "'a absval_ty_fun \<Rightarrow> 'm proc_context \<Rightarrow> var_context \<Rightarrow> 'a fun_interp \<Rightarrow> rtype_env \<Rightarrow> expr list \<Rightarrow> expr list \<Rightarrow> ast \<Rightarrow> 'a nstate \<Rightarrow> bool"
   where "proc_body_satisfies_spec A M \<Lambda> \<Gamma> \<Omega> pres posts ast ns \<equiv>
          expr_all_sat A \<Lambda> \<Gamma> \<Omega> ns pres \<longrightarrow> 
           (\<forall> bb cont state. (rtranclp (red_bigblock A M \<Lambda> \<Gamma> \<Omega> ast) (init_ast ast ns) (bb, cont, state)) \<longrightarrow> 
