BoogieLang/Passification.thy
@@ -27,7 +27,7 @@ lemma dependent_ext:
   unfolding dependent_def
   by blast
 
-definition set_red_cmd :: "'a absval_ty_fun \<Rightarrow> mbodyCFG proc_context \<Rightarrow> var_context \<Rightarrow> 'a fun_interp \<Rightarrow> rtype_env \<Rightarrow> cmd \<Rightarrow> 'a nstate set \<Rightarrow> 'a state set"
+definition set_red_cmd :: "'a absval_ty_fun \<Rightarrow> 'm proc_context \<Rightarrow> var_context \<Rightarrow> 'a fun_interp \<Rightarrow> rtype_env \<Rightarrow> cmd \<Rightarrow> 'a nstate set \<Rightarrow> 'a state set"
   where "set_red_cmd A M \<Lambda> \<Gamma> \<Omega> c N = {s. \<exists>n_s. n_s \<in> N \<and> A,M,\<Lambda>,\<Gamma>,\<Omega> \<turnstile> \<langle>c, Normal n_s\<rangle> \<rightarrow> s}"
 
 text \<open>\<^term>\<open>set_red_cmd\<close> lifts the command reduction to the reduction of a a set of input states \<close>
